\documentclass[9pt,twocolumn]{extarticle}

\usepackage[hmargin=0.5in,tmargin=0.5in]{geometry}
\usepackage{amsmath,amssymb}
\usepackage{times}

\usepackage{cleveref}
\usepackage{color}
\newcommand{\TODO}[1]{\textcolor{red}{#1}}

\newcommand{\FPP}[2]{\frac{\partial #1}{\partial #2}}
\newcommand{\argmin}{\operatornamewithlimits{arg\ min}}
\author{Siwang Li}

\title{Material Optimization using Direct Method}

%% document begin here
\begin{document}
\maketitle

\setlength{\parskip}{0.5ex}

\section{Objective function}
The objective function for minimize the control forces is
\begin{equation} \label{obj} E(z,\Lambda,\alpha_k,\alpha_m) = \frac{1}{2}\sum_{i=2}^{T-1}
  \|\frac{1}{h^2}\hat{z}_i+\frac{1}{h}D(z_{i+1}-z_{i})+ \Lambda z_i\|_2^2
\end{equation}
where $h$ is the time step, $\hat{z}_i=z_{i+1}-2z_{i}+z_{i-1}$,
$D=\alpha_mI+\alpha_k\Lambda$ is the damping. Then we apply the partial
constraints $C(z) = \frac{1}{2}\|u^j(z_i)-u_c^j\|_2^2$ using penalty method, and
apply the keyframe constraints using variables replacement, we finally obtain
the optimization problem,
\begin{eqnarray} \label{sp}
  &&\argmin_{z,\Lambda,\alpha_m,\alpha_k}E(z,\Lambda,\alpha_k,\alpha_m)+\gamma_cC(z)\\
  &&\mbox{s.t. } z_{k_i} = z'_{k_i}
\end{eqnarray}

In the following we introduce the details for the optimization of the above
problem.

\section{Optimize displacements}
\subsection{Control forces}
\begin{eqnarray*}
  E(z) &=& \frac{1}{2}\sum_{i=2}^{T-1}
  \|\frac{1}{h^2}\hat{z}_i+\frac{1}{h}D(z_{i+1}-z_{i})+ \Lambda z_i\|_2^2\\
  &=& \frac{1}{2}\sum_{i=2}^{T-1}
  \|\frac{1}{h^2}(z_{i+1}-2z_{i}+z_{i-1})+\frac{1}{h}D(z_{i+1}-z_{i})+ \Lambda
  z_i\|_2^2\\
  &=& \frac{1}{2}\sum_{i=2}^{T-1}
  \|(\frac{1}{h^2}I+\frac{1}{h}D)z_{i+1}+(\Lambda-\frac{1}{h}D-\frac{2}{h^2}I)z_i
  + \frac{1}{h^2}z_{i-1}\|_2^2\\
  Z_0 &=& (z_0,\cdots,z_{T-3})\\
  Z_1 &=& (z_1,\cdots,z_{T-2})\\
  Z_2 &=& (z_2,\cdots,z_{T-1})\\
  A &=& \frac{1}{h^2}I+\frac{1}{h}D\\
  B &=& \Lambda-\frac{1}{h}D-\frac{2}{h^2}I\\
  E(z) &=& \frac{1}{2}\|AZ_{2}+BZ_1 + \frac{1}{h^2}Z_{0}\|_2^2
\end{eqnarray*}

\begin{eqnarray*}
  a &=& A_{ii}\\
  b &=& B_{ii}\\
  c &=& \frac{1}{h^2}\\
  E(z)  &=& \frac{1}{2}\sum_{i=2}^{T-1}\|az_{i+1}+bz_i+cz_{i-1}\|_2^2
\end{eqnarray*}

\[
\left( \begin{array}{ccccccc}
    c^2&bc&ac&0&0&0&0\\
    bc&c^2+b^2&bc+ab&ac&0&0&0\\
    ac&bc+ab&c^2+b^2+a^2&bc+ab&ac&0&0\\
    0&ac&bc+ab&c^2+b^2+a^2&bc+ab&ac&0\\
    0&0&ac&bc+ab&c^2+b^2+a^2&bc+ab&ac\\
    0&0&0&ac&bc+ab&b^2+a^2&ab\\
    0&0&0&0&ac&ab&a^2\\
  \end{array} \right)
\]

\subsection{Partial Constraints}
The full RS method is equal to solve a linear system
\begin{equation} \label{rs}
  Au = b(y(z)).
\end{equation}
where $y(z) = \tilde{y} + \hat{W}z$. Let $B$ be some linear basis matrix, and
$P=(B^TAB)^{-1}B^T$, then by using the Cubature scheme, obtain
\begin{equation} \label{reduced_rs3}
  u \approx B\sum_{e\in{S}}w_eP_e{b_e(y(z))}
\end{equation}
Then we can compute the displacement $u_i(z)$ of node $i$ using
\begin{equation}
  u_i(z) = (B_iP)b(\tilde{y} + \hat{W}z)
\end{equation}
and the gradient is
\begin{equation}
  \frac{\partial{u_i}}{\partial{z}} = P_i \frac{\partial{b}}{\partial{y}}
  \hat{W} = P_i
  \left( \begin{array}{c}
      \frac{\partial{b}}{\partial{y_0}} \hat{W}_0\\
      \vdots\\
      \frac{\partial{b}}{\partial{y_N}} \hat{W}_N
    \end{array} \right)_{9N\times r_2} = 
  \sum(P_{ij}\frac{\partial{b}}{\partial{y_j}})\hat{W}_j
\end{equation}
where $P_{ij}\in R^{3\times 9}$, and
\begin{equation}
  b_j(y_j) = \sqrt{V_j}(exp(y_j^w)(I+y_j^e)-I)
\end{equation}
and $\frac{\partial{b_j}}{\partial{y_j}}$ is a $9\times9$ matrix. Finally we
compute 
\begin{equation} \label{compPePz}
  {\frac{\partial{E}}{\partial{z_i}}} =
  (\frac{\partial{u}}{\partial{z_i}})^Tu' =
  \sum\hat{W}_j^T(\frac{\partial{b}}{\partial{y_j}})^TP_{ij}^Tu'
\end{equation}
where $u' = C^TCu-C^Tu^c$.

\section{Optimize materials}
\subsection{Objective function}
\begin{eqnarray*}
  Z_0 &=& (z_0,\cdots,z_{T-3})\\
  Z_1 &=& (z_1,\cdots,z_{T-2})\\
  Z_2 &=& (z_2,\cdots,z_{T-1})\\
  \tilde{Z}_2 &=& \frac{1}{h}(Z_2-Z_1)\\
  \hat{Z}_2 &=& \frac{1}{h^2}(Z_2-2Z_1+Z_0)\\
  D &=& \alpha_mI+\alpha_kK\\
  E(\alpha_m,\alpha_k,K)&=&\frac{1}{2}\|\hat{Z}_2+D\tilde{Z}_2+KZ_1\|_2^2
\end{eqnarray*}

\subsection{Gradient}
\begin{eqnarray*}
  E &=& \tilde{Z}_2 \\
  F &=& \hat{Z}_2+\alpha_kK\tilde{Z}_2+KZ_1\\
  \Phi &=& \frac{1}{2}\|\alpha_mE+F\|_2^2 \\
  &=&\frac{1}{2}(\alpha_mE_{i{ }j}+F_{i{ }j})^2\\
  \frac{\partial{\Phi}}{\partial{\alpha_m}} &=&
  E_{i{ }j}(\alpha_mE_{i{ }j}+F_{i{ }j})\\
  &=&E:(\alpha_mE+F)\\
  G &=& K\tilde{Z}_2\\
  H &=& \hat{Z}_2+\alpha_m\tilde{Z}_2+KZ_1\\
  \Phi &=& \frac{1}{2}\|\alpha_kG+H\|_2^2\\
  \frac{\partial{\Phi}}{\partial{\alpha_k}} &=&G:(\alpha_kG+H)
\end{eqnarray*}

\begin{eqnarray*}
  K &=& A^TA\\
  J &=& \alpha_k\\
  L &=& Z_1\\
  M &=& \hat{Z}_2+\alpha_m\tilde{Z}_2\\
  \Phi &=& \frac{1}{2}\| J(A^TA)E + (A^TA)L + M \|_2^2\\
  \Phi &=& \frac{1}{2}(A_{si}A_{st}L_{th}+A_{lj}A_{lk}J_{ik}E_{jh}+M_{ih})^2\\
  \frac{\partial{\Phi}}{\partial{A_{xy}}}
  &=&A_{st}L_{th}(A_{si}A_{st}L_{th}+A_{lj}A_{lk}J_{ik}E_{jh}+M_{ih})\delta_x^s\delta_y^i+\\
  &&A_{si}L_{th}(A_{si}A_{st}L_{th}+A_{lj}A_{lk}J_{ik}E_{jh}+M_{ih})\delta_x^s\delta_y^t+\\
  &&A_{lk}J_{ik}E_{jh}(A_{si}A_{st}L_{th}+A_{lj}A_{lk}J_{ik}E_{jh}+M_{ih})\delta_x^l\delta_y^j+\\
  &&A_{lj}J_{ik}E_{jh}(A_{si}A_{st}L_{th}+A_{lj}A_{lk}J_{ik}E_{jh}+M_{ih})\delta_x^l\delta_y^k\\
  &=&A_{xt}L_{th}(A_{xy}A_{xt}L_{th}+A_{lj}A_{lk}J_{yk}E_{jh}+M_{yh})+\\
  &&A_{xi}L_{yh}(A_{xi}A_{xy}L_{yh}+A_{lj}A_{lk}J_{ik}E_{jh}+M_{ih})+\\
  &&A_{xk}J_{ik}E_{yh}(A_{si}A_{st}L_{th}+A_{xy}A_{xk}J_{ik}E_{yh}+M_{ih})+\\
  &&A_{xj}J_{iy}E_{jh}(A_{si}A_{st}L_{th}+A_{xj}A_{xy}J_{iy}E_{jh}+M_{ih})\\
  &=&  (AL)_{xh}((A^TAL)_{yh}+(E^TA^TAJ^T)_{hy}+M_{yh})+\\
  &&A_{xi}L_{yh}((A^TAL)_{ih}+(E^TA^TAJ^T)_{hi}+M_{ih})+\\
  &&(AJ^T)_{xi}E_{yh}((A^TAL)_{ih}+(E^TA^TAJ^T)_{hi}+M_{ih})+\\
  &&(AE)_{xh}J_{iy}((A^TAL)_{ih}+(E^TA^TAJ^T)_{hi}+M_{ih})\\
  &=& ((A^TALL^TA^T)_{yx}+(ALE^TA^TAJ^T)_{xy}+(ALM^T)_{xy})+\\
  &&((AA^TALL^T)_{xy}+(LE^TA^TAJ^TA^T)_{yx}+(AML^T)_{xy})+\\
  &&((AJ^TA^TALE^T)_{xy}+(EE^TA^TAJ^TJA^T)_{yx}+\\
  &&(AJ^TME^T)_{xy})+\\
  &&((J^TA^TALE^TA^T)_{yx}+(AEE^TA^TAJ^TJ)_{xy}+(AEM^TJ)_{xy})
\end{eqnarray*}


%% references
% \begin{thebibliography}{99}
% \bibitem{sig2011} Fast simulation of skeleton-driven deformable body
%   characters.
% \end{thebibliography}

\end{document}
